examples: dm4f: tidy up all around
I broke some exmamples, but I think it's a step forward.

examples/dm4free/FStar.DM4F.Exceptions.fst
@@ -1,19 +1,30 @@
 module FStar.DM4F.Exceptions
 
-let ex (a:Type) = 
-  unit -> M (option a)
+(**********************************************************
+ * Dijkstra Monads for Free : Exceptions
+ *
+ * Example of an exception monad effect, with a lift from
+ * the Pure effect into it and an example of how both
+ * intrinsic and extrinsic proof methods can be used
+ * on a simple division function.
+ *
+ **********************************************************)
 
-val return_ex : a:Type -> x:a -> ex a
+(* The underlying representation type *)
+let ex (a:Type) = unit -> M (option a)
+
+(* Monad definition *)
+val return_ex : (a:Type) -> (x:a) -> ex a
 let return_ex a x = fun _ -> Some x
 
-val bind_ex : a:Type -> b:Type -> f:ex a -> g:(a -> ex b) -> ex b
-let bind_ex a b f g = fun _ -> 
-  let r = f () in 
-  match r with 
+val bind_ex : (a:Type) -> (b:Type) -> (f:ex a) -> (g:a -> ex b) -> ex b
+let bind_ex a b f g = fun _ ->
+  let r = f () in
+  match r with
   | None -> None
   | Some x -> g x ()
 
-(* #set-options "--debug FStar.DM4F.Exceptions --debug_level Extreme --print_universes --print_implicits" *)
+(* Define the new effect using DM4F *)
 reifiable reflectable new_effect_for_free {
   EXN : a:Type -> Effect
   with
@@ -22,30 +33,64 @@ reifiable reflectable new_effect_for_free {
   ; return       = return_ex
 }
 
+(* Logical types, derived from the effect definition. *)
+let ex_pre  = EXN.pre
+let ex_post = EXN.post
+let ex_wp   = EXN.wp
+let ex_repr = EXN.repr
 
-let ex_pre = Type0
-let ex_post (a:Type) = option a -> Type0
-let ex_wp (a:Type) = unit -> ex_post a -> Type0
-
+(* A lift from `Pure´ into the new effect *)
 inline let lift_pure_ex (a:Type) (wp:pure_wp a) (_:unit) (p:ex_post a) = wp (fun a -> p (Some a))
 sub_effect PURE ~> EXN = lift_pure_ex
 
-effect Exn (a:Type) (pre:ex_pre) (post:ex_post a) =
+(* An effect to alias easily write pre- and postconditions *)
+(* Note: we use Type0 instead of ex_pre to avoid having to thunk everything. *)
+effect Exn (a:Type) (pre:Type0) (post:ex_post a) =
        EXN a
-         (fun (_:unit) (p:ex_post a) -> pre /\ (forall (r:option a). (pre /\ post r) ==> p r)) (* WP *)
+         (fun (_:unit) (p:ex_post a) -> pre /\ (forall (r:option a). (pre /\ post r) ==> p r))
 
-effect Ex (a:Type) = //(pre:ex_pre) (post:ex_post a) ...adding this mistakenly causes a crash!
+(* Another alias. Ex a is the effect type for total exception-throwing
+ * programs. i.e. Any program of type `Ex a´ will throw or finish
+ * correctly, but never loop. *)
+effect Ex (a:Type) =
        EXN a (fun _ p -> forall x. p x)
 
-let ex_repr (a:Type) (wp:ex_wp a) =
-    unit -> PURE (option a) (wp ())
-
+(*
+ * We can also build a new action "on the fly" using reflect!
+ * Here we define raise_ as a pure function working with the
+ * representation of Ex.
+ *)
 val raise_ : a:Type -> Tot (ex_repr a (fun (_:unit) (p:ex_post a) -> p None))
 let raise_ a (_:unit) = None
 
-//You can also build a new action "on the fly" using reflect
-reifiable let raise (a:Type) : Exn a True (fun r -> r==None)
+(* We reflect it back to Exn *)
+reifiable let raise (a:Type) : Exn a True (fun r -> r == None)
   = EXN.reflect (raise_ a)
+
+(*
+ * We now show `div´ to be correct in two ways. The property we show is
+ * that if `div´ throws, then the divisor was zero; and if it doesn't,
+ * then the divisor was not zero and the result (z) is the division of i
+ * and j.
+ *
+ * In the first definition, we give a strong type to `div´: we make use
+ * of `Exn´ to give pre- and postconditions to the function, specifying
+ * the property we want. This is known as an intrinsic proof: it's
+ * within the definition.
+ *
+ * In the second, we give a very lax type to div, namely `Ex int´ (note
+ * it is different from Exn). This type is only implying that calling
+ * div will either throw an exception or return an int, but there's no
+ * specification about the result or about when exceptions occur.
+ *
+ * As `Ex´ is a reifiable effect, we can reason about `div´ outside of
+ * its definition by turning it into a pure function. This is what is
+ * done in the `lemma_div_extrinsic´ lemma.
+ *
+ * For primitive effects, this is impossible since logical properties
+ * (in proof-irrelevant contexts) only make sense for pure and total
+ * terms, so one is only able to do proofs intrinsically.
+ *)
 
 val div_intrinsic : i:nat -> j:int -> Exn int
   (requires True)
@@ -61,5 +106,4 @@ reifiable let div_extrinsic (i:nat) (j:int) : Ex int =
 let lemma_div_extrinsic (i:nat) (j:int) :
   Lemma (match reify (div_extrinsic i j) () with
          | None -> j = 0
-	 | Some z -> j <> 0 /\ z = i / j) = ()
-
+         | Some z -> j <> 0 /\ z = i / j) = ()
