examples/dm4free/FStar.DM4F.ST.fst
@@ -1,28 +1,41 @@
 module FStar.DM4F.ST
 
-// Note: being in the [FStar] namespace, only [Prims] is automatically opened
-// for the current module.
+(**********************************************************
+ * Dijkstra Monads for Free : Simple state
+ *
+ * A minimal example of defining a state effect along
+ * with actions, over a parametrized state type.
+ *
+ **********************************************************)
 
-let st (h: Type) (a: Type) =
+(* The underlying representation type *)
+let st (h:Type) (a:Type) =
   h -> M (a * h)
 
-val return_st: h:Type -> a:Type -> x:a -> st h a
+(* Monad definition *)
+val return_st : (h:Type) -> (a:Type) -> a -> st h a
 let return_st h a x = fun s -> x, s
 
-val bind_st: h:Type -> a:Type -> b:Type -> f:st h a -> g:(a -> st h b) -> st h b
+val bind_st: (h:Type) -> (a:Type) -> (b:Type) ->
+             st h a -> (a -> st h b) -> st h b
 let bind_st h a b f g = fun s0 ->
   let tmp = f s0 in
   let x, s1 = tmp in
   g x s1
 
-let get (h: Type) (_:unit): st h h =
+(* Actions (get is thunked) *)
+let get (h:Type) (_:unit): st h h =
   fun x -> x, x
 
 let put (h: Type) (x: h): st h unit =
   fun _ -> (), x
 
+(*
+ * Do the DM4F work. Note that the heap type is a parameter
+ * of the resulting effect.
+ *)
 reifiable reflectable new_effect_for_free {
-  STATE (h: Type): a:Type -> Effect
+  STATE (h:Type): a:Type -> Effect
   with repr     = st h
      ; bind     = bind_st h
      ; return   = return_st h
