examples/dm4free/FStar.DM4F.StExnC.fst
@@ -1,0 +1,108 @@
+module FStar.DM4F.StExn
+
+(**********************************************************
+ * Dijkstra Monads for Free : State with exceptions
+ *
+ * State over exceptions (state kept when raising).
+ *
+ * We don't define a get and put, but instead use the state
+ * for counting the amount of exceptions thrown.
+ *
+ **********************************************************)
+
+(* TODO: parametrize heap? *)
+
+(* The underlying representation type. The two ints are
+ * resulting state and exception count, respectively. *)
+let stexn a =
+  int -> M (option a * (int * int))
+
+(* Monad definition *)
+val return : (a:Type) -> (x:a) -> stexn a
+let return a x = fun s -> Some x, (s, 0)
+
+val bind : (a:Type) -> (b:Type) ->
+           (f:stexn a) -> (g:a -> stexn b) -> stexn b
+let bind a b f g =
+  fun s0 ->
+    (* TODO: need to letbind f s0 to match on it; expected? idem grs1 *)
+    let fs0 = f s0 in
+    match fs0 with
+    | None, (s1, c1) -> None, (s1, c1)
+    | Some r, (s1, c1) -> let grs1 = g r s1 in
+                          match grs1 with
+                          | res, (s, c2) -> res, (s, c1 + c2)
+
+let put (s:int) : stexn unit =
+        fun s0 -> (Some (), (s0, 0))
+
+let get (_:unit) : stexn int =
+        fun s0 -> (Some s0, (s0, 0))
+
+(* Same error as StExn *)
+let raise (a:Type) : stexn a =
+        fun s0 -> (None, (s0, 1))
+
+(*
+ * Define the new effect using DM4F. We don't mark it as reflectable
+ * so we know the invariant of exception-counting is enforced
+ *)
+reifiable new_effect_for_free {
+  STEXN: a:Type -> Effect
+  with repr = stexn
+     ; return = return
+     ; bind = bind
+  and effect_actions
+       put = put
+     ; get = get
+     ; raise = raise
+}
+
+let pre  = STEXN.pre
+let post = STEXN.post
+let wp   = STEXN.wp
+let repr = STEXN.repr
+
+(* A lift from Pure *)
+inline let lift_pure_stexn (a:Type) (wp:pure_wp a) (h0:int) (p:post a) =
+        wp (fun a -> p (Some a, (h0, 0)))
+sub_effect PURE ~> STEXN = lift_pure_stexn
+
+(* NOTE: no lift from IntST.STATE to StateExn, since that would break
+         the abstraction of counting exceptions *)
+
+(* TODO: but why? there are no exception in IntST. Maybe StExn is meant?  *)
+
+(* Pre-/postcondition variant *)
+effect StExn (a:Type) (req:pre) (ens:int -> option a -> int -> int -> GTot Type0) =
+       STEXN a
+         (fun (h0:int) (p:post a) -> req h0
+          /\ (forall (r:option a) (h1:int) (c:int).
+                 (req h0 /\ ens h0 r h1) ==> p (r, (h1, c))))
+
+(* Total variant *)
+effect S (a:Type) =
+       STEXN a (fun h0 p -> forall x. p x)
+
+(* This rightfully fails, since StateExn is not reflectable *)
+
+// reifiable let f (a:Type) : STEXN a (fun h0 post -> post (None, h0)) =
+//         STEXN.reflect (fun h0 -> None, h0)
+
+val div_intrinsic : i:nat -> j:int -> StExn int
+  (requires (fun h -> True))
+  (ensures (fun h0 x h1 -> match x with
+                        | None -> h0 + 1 = h1 /\ j=0
+                        | Some z -> h0 = h1 /\ j<>0 /\ z = i / j))
+let div_intrinsic i j =
+  if j=0 then raise int
+  else i / j
+
+reifiable let div_extrinsic (i:nat) (j:int) : S int =
+  if j=0 then raise int
+  else i / j
+
+let lemma_div_extrinsic (i:nat) (j:int) :
+  Lemma (match reify (div_extrinsic i j) 0 with
+         | None, 1 -> j = 0
+         | Some z, 0 -> j <> 0 /\ z = i / j) = ()
